wp4: proof update

examples/hoare_logic/wp4/wp4_ImpExpr_eval_subst_term_1.v
@@ -33,11 +33,13 @@ Inductive operator  :=
 (* Why3 assumption *)
 Definition ident  := Z.
 
+Parameter refident : Type.
+
 (* Why3 assumption *)
 Inductive term  :=
   | Tvalue : value -> term 
   | Tvar : Z -> term 
-  | Tderef : Z -> term 
+  | Tderef : refident -> term 
   | Tbin : term -> operator -> term -> term .
 
 (* Why3 assumption *)
@@ -65,16 +67,16 @@ Axiom Select_neq : forall (a:Type) (b:Type), forall (m:(map a b)),
   forall (a1:a) (a2:a), forall (b1:b), (~ (a1 = a2)) -> ((get (set m a1 b1)
   a2) = (get m a2)).
 
-Parameter const: forall (b:Type) (a:Type), b -> (map a b).
+Parameter const: forall (a:Type) (b:Type), b -> (map a b).
 Set Contextual Implicit.
 Implicit Arguments const.
 Unset Contextual Implicit.
 
-Axiom Const : forall (b:Type) (a:Type), forall (b1:b) (a1:a),
+Axiom Const : forall (a:Type) (b:Type), forall (b1:b) (a1:a),
   ((get (const b1:(map a b)) a1) = b1).
 
 (* Why3 assumption *)
-Definition env  := (map Z value).
+Definition env  := (map refident value).
 
 (* Why3 assumption *)
 Inductive list (a:Type) :=
@@ -112,9 +114,16 @@ Axiom get_stack_def : forall (i:Z) (pi:(list (Z* value)%type)),
       ((get_stack i pi) = (get_stack i r)))
   end.
 
+Axiom get_stack_eq : forall (x:Z) (v:value) (r:(list (Z* value)%type)),
+  ((get_stack x (Cons (x, v) r)) = v).
+
+Axiom get_stack_neq : forall (x:Z) (i:Z) (v:value) (r:(list (Z*
+  value)%type)), (~ (x = i)) -> ((get_stack i (Cons (x, v) r)) = (get_stack i
+  r)).
+
 (* Why3 assumption *)
 Set Implicit Arguments.
-Fixpoint eval_term(sigma:(map Z value)) (pi:(list (Z* value)%type))
+Fixpoint eval_term(sigma:(map refident value)) (pi:(list (Z* value)%type))
   (t:term) {struct t}: value :=
   match t with
   | (Tvalue v) => v
@@ -127,7 +136,7 @@ Unset Implicit Arguments.
 
 (* Why3 assumption *)
 Set Implicit Arguments.
-Fixpoint eval_fmla(sigma:(map Z value)) (pi:(list (Z* value)%type))
+Fixpoint eval_fmla(sigma:(map refident value)) (pi:(list (Z* value)%type))
   (f:fmla) {struct f}: Prop :=
   match f with
   | (Fterm t) => ((eval_term sigma pi t) = (Vbool true))
@@ -144,15 +153,26 @@ Fixpoint eval_fmla(sigma:(map Z value)) (pi:(list (Z* value)%type))
   end.
 Unset Implicit Arguments.
 
-Parameter subst_term: term -> Z -> Z -> term.
+Parameter subst_term: term -> refident -> Z -> term.
 
-Axiom subst_term_def : forall (e:term) (r:Z) (v:Z),
+Axiom subst_term_def : forall (e:term) (r:refident) (v:Z),
   match e with
   | ((Tvalue _)|(Tvar _)) => ((subst_term e r v) = e)
   | (Tderef x) => ((r = x) -> ((subst_term e r v) = (Tvar v))) /\
       ((~ (r = x)) -> ((subst_term e r v) = e))
   | (Tbin e1 op e2) => ((subst_term e r v) = (Tbin (subst_term e1 r v) op
       (subst_term e2 r v)))
+  end.
+
+Parameter vsubst_term: term -> Z -> term -> term.
+
+Axiom vsubst_term_def : forall (e:term) (v:Z) (t:term),
+  match e with
+  | ((Tvalue _)|(Tderef _)) => ((vsubst_term e v t) = e)
+  | (Tvar x) => ((v = x) -> ((vsubst_term e v t) = t)) /\ ((~ (v = x)) ->
+      ((vsubst_term e v t) = e))
+  | (Tbin e1 op e2) => ((vsubst_term e v t) = (Tbin (vsubst_term e1 v t) op
+      (vsubst_term e2 v t)))
   end.
 
 (* Why3 assumption *)
@@ -167,19 +187,19 @@ Fixpoint fresh_in_term(id:Z) (t:term) {struct t}: Prop :=
 Unset Implicit Arguments.
 
 (* Why3 goal *)
-Theorem eval_subst_term : forall (sigma:(map Z value)) (pi:(list (Z*
-  value)%type)) (e:term) (x:Z) (v:Z), (fresh_in_term v e) ->
+Theorem eval_subst_term : forall (sigma:(map refident value)) (pi:(list (Z*
+  value)%type)) (e:term) (x:refident) (v:Z), (fresh_in_term v e) ->
   ((eval_term sigma pi (subst_term e x v)) = (eval_term (set sigma x
   (get_stack v pi)) pi e)).
-induction e; intros r v' H.
+induction e; intros x v' H.
 
-rewrite (subst_term_def (Tvalue v) r v'); auto.
+rewrite (subst_term_def (Tvalue v) x v'); auto.
 
-rewrite (subst_term_def (Tvar z) r v'); auto.
+rewrite (subst_term_def (Tvar z) x v'); auto.
 
-generalize (subst_term_def (Tderef z) r v').
+generalize (subst_term_def (Tderef r) x v').
 intros (h1,h2).
-case (Z_eq_dec r z).
+case (Z_eq_dec x r).
 intro; subst r; rewrite h1; simpl; auto.
 rewrite Select_eq; auto.
 intro; rewrite h2; simpl; auto.
